# Chapter 04

### Ray-Sphere Intersection

(x - C<sub>x</sub>)<sup>2</sup> + (y - C<sub>y</sub>)<sup>2</sup> + (z - C<sub>z</sub>)<sup>2</sup> = r<sup>2</sup>

<=> (**P** - **C**) &sdot; (**P** - **C**) = r<sup>2</sup>

<=> (**A** + t**b** - C) &sdot; (**A** + t**b** - C) = r<sup>2</sup>

<=> t<sup>2</sup>**b**&sdot;**b** + 2t**b** &sdot; (A - C) + (A - C) &sdot; (A - C) - r<sup>2</sup> = 0

![fig.ray-sphere](note images/fig.ray-sphere.jpg)



### Output Display

A simple red sphere

![output](output.png)

